src/lowparse/pulse/LowParse.PulseParse.Sum.fst
@@ -3151,7 +3151,20 @@ let l2r_safe_writer_dsum_noroom_lemma
     Seq.lemma_len_append
       (serialize (serialize_maybe_enum_key _ s (dsum_enum t)) tg)
       (serialize (serialize_dsum_cases t f sr g sg tg) yh);
-    assert (Seq.length (serialize (serialize_maybe_enum_key _ s (dsum_enum t)) k) == SZ.v tag_sz)
+    assert (Seq.length (serialize (serialize_maybe_enum_key _ s (dsum_enum t)) k) == SZ.v tag_sz);
+    assert (dsum_conv t mid_of_tag conv_of_tag m == Some yh);
+    assert (serialize (serialize_dsum t s f sr g sg) yh ==
+      Seq.append
+        (serialize (serialize_maybe_enum_key _ s (dsum_enum t)) tg)
+        (serialize (serialize_dsum_cases t f sr g sg tg) yh));
+    assert (tg == k);
+    Seq.lemma_len_append
+      (serialize (serialize_maybe_enum_key _ s (dsum_enum t)) tg)
+      (serialize (serialize_dsum_cases t f sr g sg tg) yh);
+    assert (Seq.length (serialize (serialize_dsum t s f sr g sg) yh) ==
+      Seq.length (serialize (serialize_maybe_enum_key _ s (dsum_enum t)) tg) +
+      Seq.length (serialize (serialize_dsum_cases t f sr g sg tg) yh));
+    assert (Seq.length (serialize (serialize_dsum t s f sr g sg) yh) >= SZ.v tag_sz)
 
 inline_for_extraction
 fn l2r_safe_writer_dsum
